Saving

semantics/programs.v
@@ -61,7 +61,7 @@ Definition append_write (W1 W2: the_write_stuff) :=
 (*steps to termination, accumulates write data*)
 
 (*continuous traces*)
-Notation step :=((context * context * obseq) * the_write_stuff).
+Notation step :=(context * context * obseq).
 
  Fixpoint last {A: Type} (l:list A) :=
   match l with
@@ -96,16 +96,16 @@ Qed. *)
  Definition getstart (T: (list step) * context * context) := match T with
                                                              (out, _, _) => out end. *)
 (*steps, start, end*)
-Inductive trace_c: (list step) -> context -> context -> Type :=
-  CTrace_Empty: forall(C: context), trace_c [((C, C, nil), emptysets)] C C
+Inductive trace_c: (list step) -> context -> context -> the_write_stuff -> Type :=
+  CTrace_Empty: forall(C: context), trace_c [] C C emptysets
 | CTrace_single: forall {C1 C2: context} {O: obseq} {W: the_write_stuff},
                   cceval_w C1 O C2 W -> (*command in C2 is skip by def single_com, cceval_w*)
-                  trace_c [((C1, C2, O), W)] C1 C2
-| CTrace_App: forall{L1 L2: list step} {S1 E1 S2 E2: context},
-               trace_c L1 S1 E1 ->
-               trace_c L2 S2 E2->
+                  trace_c [(C1, C2, O)] C1 C2 W
+| CTrace_App: forall{L1 L2: list step} {W1 W2: the_write_stuff} {S1 E1 S2 E2: context},
+               trace_c L1 S1 E1 W1->
+               trace_c L2 S2 E2 W2->
                E1 = S2 ->
-               trace_c (L1 ++ L2) S1 E2.
+               trace_c (L1 ++ L2) S1 E2 (append_write W1 W2).
 
 
 (*intermittent traces*)
@@ -127,33 +127,33 @@ iTrace_Empty: forall{C: iconf},
 Definition multi_step_c (C1 C2: context) (O: obseq) :=
     exists W: the_write_stuff, inhabited (trace_c C1 C2 O W). *)
 
-Definition multi_step_c (C1 C2: context) :=
-  exists (L: list step), inhabited (trace_c L C1 C2).
-
-Definition multi_step_i (C1 C2: iconf) (O: obseq) :=
-    exists W: the_write_stuff, trace_i C1 C2 O W.
 (*more trace helpers*)
 
-Fixpoint acc_wts (L: list step) :=
+(*Fixpoint acc_wts (L: list step) :=
   match L with
     [] => emptysets
-  |(((_, _, _), W1):: xs) => append_write W1 (acc_wts xs) end.
+  |(((_, _, _), W1):: xs) => append_write W1 (acc_wts xs) end.*)
 
 Fixpoint acc_obs (L: list step) :=
   match L with
     [] => []
-  |(((_, _, obs), _):: xs) => obs ++ (acc_obs xs) end.
+  |((_, _, obs):: xs) => obs ++ (acc_obs xs) end.
 
-Definition Wt {C1 C2: context} {L: list step} (T: trace_c L C1 C2) :=
-getwt (acc_wts L).
+Definition Wt {C1 C2: context} {L: list step} {W: the_write_stuff} (T: trace_c L C1 C2 W) :=
+getwt W.
 
-Definition FstWt {C1 C2: context} {L: list step} (T: trace_c L C1 C2)
-            := getfstwt (acc_wts L).
-Definition getobs {C1 C2: context} {L: list step} (T: trace_c L C1 C2) :=
+Definition FstWt {C1 C2: context} {L: list step} {W: the_write_stuff} (T: trace_c L C1 C2 W)
+            := getfstwt W.
+Definition getobs {C1 C2: context} {L: list step} {W: the_write_stuff} (T: trace_c L C1 C2 W) :=
   acc_obs L.
 
 (**********************************************************************************)
 
+Definition multi_step_c (C1 C2: context) (O: obseq)  :=
+  exists (L: list step) (W: the_write_stuff) (T: trace_c L C1 C2 W), (getobs T) = O.
+
+Definition multi_step_i (C1 C2: iconf) (O: obseq) :=
+    exists W: the_write_stuff, trace_i C1 C2 O W.
 
 (*relations between continuous and intermittent memory*)
 
@@ -171,15 +171,16 @@ Definition getobs {C1 C2: context} {L: list step} (T: trace_c L C1 C2) :=
 Lemma refl_context : forall (C1: context), C1 = C1.
 intros. reflexivity. Qed. 
 
+(*what about a relation for when there's not a checkpoint left?*)
 Inductive same_pt: nvmem -> vmem -> command -> command -> nvmem -> nvmem -> Prop:=
 same_mem: forall {N0 N1 N2 Ncomp: nvmem}
                   {V0 V1 V2: vmem}
-                  {c0 c1: command}
+                  {c0 c1 c2: command}
                   {w: warvars}
                   {L1 L2: list step}
-                  (T1: trace_c L1 (N0, V0, c0) (N1, V1, c1))
-                  (T2: trace_c L2 (N1, V1, c1) (N2, V2, Ins (incheckpoint w))),
-                  (getdomain N1) = (getdomain Ncomp) 
+                  {W1 W2: the_write_stuff}
+                  (T1: trace_c L1 (N0, V0, c0) (N1, V1, c1) W1 )
+                  (T2: trace_c L2 (N1, V1, c1) (N2, V2, (incheckpoint w);; c2) W2), (*c2 could be skip*)      (getdomain N1) = (getdomain Ncomp) 
                   -> not (In checkpoint (getobs T1))
                   -> not (In checkpoint (getobs T2)) (*checks checkpoint T2 ends on is nearest checkpoint*)
                  -> (forall(l: loc),
@@ -194,13 +195,13 @@ N is state of checkpoint at N1
  V1 isn't used anywhere it's just to fill out the type
  N2, V2 is final state for intermittent, once again solely to fill out the type*)
 Inductive current_init_pt: nvmem -> vmem -> command -> nvmem -> nvmem -> Prop:=
-valid_mem: forall {N N0 N1: nvmem}
-                  {V0 V1: vmem}
-                  {c: command}
+valid_mem: forall {N N0 N1 N2: nvmem}
+                  {V0 V1 V2: vmem}
+                  {c c1: command}
                   {w: warvars}
                   {L: list step}
-                  {C2: context}
-                  (T: trace_c L (N1, V1, c) C2),
+                  {W: the_write_stuff}
+                  (T: trace_c L (N1, V1, c) (N2, V2, (incheckpoint w) ;; c1 ) W),
                   (getdomain N1) = (getdomain N0) 
                   -> not (In checkpoint (getobs T)) (*checks checkpoint T ends on is nearest checkpoint*)
                  -> (forall(l: loc),
